rutt: swapping order of constructors and couple of simplifications

theories/Eq/Rutt.v
@@ -25,7 +25,6 @@ From ITree Require Import
      ITreeFacts
 .
 
-
 From Paco Require Import paco.
 
 Import Monads.
@@ -34,56 +33,51 @@ Local Open Scope monad_scope.
 
 Section RuttF.
 
-Context {E1 E2 : Type -> Type}.
-Context {R1 R2 : Type}.
-(* From the point of view of relational parametricity, it would be more fitting
+  Context {E1 E2 : Type -> Type}.
+  Context {R1 R2 : Type}.
+  (* From the point of view of relational parametricity, it would be more fitting
   to replace [(REv, RAns)] with one [REv : forall A1 A2, (A1 -> A2 -> Prop) -> (E1 A1 -> E2 A2 -> Prop)].
   Contributions to that effect are welcome. *)
-Context (REv : forall (A B : Type), E1 A -> E2 B -> Prop ).
-Context (RAns : forall (A B : Type), E1 A -> A -> E2 B -> B -> Prop ).
-Context (RR : R1 -> R2 -> Prop).
-Arguments REv {A} {B}.
-Arguments RAns {A} {B}.
+  Context (REv : forall (A B : Type), E1 A -> E2 B -> Prop ).
+  Context (RAns : forall (A B : Type), E1 A -> A -> E2 B -> B -> Prop ).
+  Context (RR : R1 -> R2 -> Prop).
+  Arguments REv {A} {B}.
+  Arguments RAns {A} {B}.
 
-Inductive ruttF
-          (vclo : (itree E1 R1 -> itree E2 R2 -> Prop) -> itree E1 R1 -> itree E2 R2 -> Prop)
-          (sim : itree E1 R1 -> itree E2 R2 -> Prop) : itree' E1 R1 -> itree' E2 R2 -> Prop :=
-  | EqRet : forall (r1 : R1) (r2 : R2), RR r1 r2 -> ruttF vclo sim (RetF r1) (RetF r2)
-  | EqTau : forall (m1 : itree E1 R1) (m2 : itree E2 R2), sim m1 m2 -> ruttF vclo sim (TauF m1) (TauF m2)
-  | EqTauL : forall (t1 : itree E1 R1) (ot2 : itree' E2 R2),
-      ruttF vclo sim (observe t1) ot2 -> ruttF vclo sim (TauF t1) ot2
-  | EqTauR : forall (ot1 : itree' E1 R1) (t2 : itree E2 R2),
-      ruttF vclo sim ot1 (observe t2) -> ruttF vclo sim ot1 (TauF t2)
+  Inductive ruttF (sim : itree E1 R1 -> itree E2 R2 -> Prop) : itree' E1 R1 -> itree' E2 R2 -> Prop :=
+  | EqRet : forall (r1 : R1) (r2 : R2),
+      RR r1 r2 ->
+      ruttF sim (RetF r1) (RetF r2)
+  | EqTau : forall (m1 : itree E1 R1) (m2 : itree E2 R2),
+      sim m1 m2 ->
+      ruttF sim (TauF m1) (TauF m2)
   | EqVis : forall (A B : Type) (e1 : E1 A) (e2 : E2 B ) (k1 : A -> itree E1 R1) (k2 : B -> itree E2 R2),
       REv e1 e2 ->
-      (forall (a : A) (b : B), RAns e1 a e2 b -> vclo sim (k1 a) (k2 b) : Prop) -> ruttF vclo sim (VisF e1 k1) (VisF e2 k2).
-Hint Constructors ruttF.
+      (forall (a : A) (b : B), RAns e1 a e2 b -> sim (k1 a) (k2 b)) ->
+      ruttF sim (VisF e1 k1) (VisF e2 k2)
+  | EqTauL : forall (t1 : itree E1 R1) (ot2 : itree' E2 R2),
+      ruttF sim (observe t1) ot2 ->
+      ruttF sim (TauF t1) ot2
+  | EqTauR : forall (ot1 : itree' E1 R1) (t2 : itree E2 R2),
+      ruttF sim ot1 (observe t2) ->
+      ruttF sim ot1 (TauF t2).
+  Hint Constructors ruttF : core.
 
-Definition rutt_ (vclo : (itree E1 R1 -> itree E2 R2 -> Prop) -> itree E1 R1 -> itree E2 R2 -> Prop )
-           (sim : itree E1 R1 -> itree E2 R2 -> Prop) (t1 : itree E1 R1) (t2 : itree E2 R2) :=
-  ruttF vclo sim (observe t1) (observe t2).
-Hint Unfold rutt_.
-Lemma rutt_monot (vclo : (itree E1 R1 -> itree E2 R2 -> Prop) -> itree E1 R1 -> itree E2 R2 -> Prop):
-  (monotone2 vclo) -> monotone2 (rutt_ vclo).
-Proof.
-  intros. red in H. red. intros. red. red in IN. induction IN; eauto.
-Qed.
+  Definition rutt_ (sim : itree E1 R1 -> itree E2 R2 -> Prop)
+             (t1 : itree E1 R1) (t2 : itree E2 R2) :=
+    ruttF sim (observe t1) (observe t2).
+  Hint Unfold rutt_ : core.
 
+  Lemma rutt_monot : monotone2 rutt_.
+  Proof.
+    red. intros. red; induction IN; eauto.
+  Qed.
 
-
-Lemma rutt_id_monot : monotone2 (@id (itree E1 R1 -> itree E2 R2 -> Prop) ).
-Proof. auto. Qed.
-
-
-
-Definition rutt : itree E1 R1 -> itree E2 R2 -> Prop := paco2 (rutt_ id) bot2.
+  Definition rutt : itree E1 R1 -> itree E2 R2 -> Prop := paco2 rutt_ bot2.
 
 End RuttF.
 
-
-Hint Resolve rutt_monot : paco.
-
-Hint Resolve rutt_id_monot : paco.
+#[export] Hint Resolve rutt_monot : paco.
 
 Lemma rutt_inv_tauL {E1 E2 R1 R2 REv RAns RR} t1 t2 :
   @rutt E1 E2 R1 R2 REv RAns RR (Tau t1) t2 -> rutt REv RAns RR t1 t2.
@@ -119,53 +113,55 @@ Proof.
 Qed.
 
 Lemma rutt_inv_tauLR  {E1 E2 R1 R2 REv RAns RR} t1 t2 :
-   @rutt E1 E2 R1 R2 REv RAns RR (Tau t1) (Tau t2) -> rutt REv RAns RR t1 t2.
+  @rutt E1 E2 R1 R2 REv RAns RR (Tau t1) (Tau t2) -> rutt REv RAns RR t1 t2.
 Proof.
   intros; apply rutt_inv_tauR, rutt_inv_tauL; assumption.
 Qed.
 
-Section eqitC_rutt.
+Section euttge_trans_clo.
+
   Context {E1 E2 : Type -> Type} {R1 R2 : Type} (RR : R1 -> R2 -> Prop).
-  (* Question, is it a problem that I don't have the booleans, is that necessary?
-     Would be simple to add but would necessitate some busy work *)
+
+  (* Closing a relation over itrees under [euttge].
+     Essentially the same closure as [eqit_trans_clo], but heterogeneous
+     in the interface argument [E].
+     We only define the closure under [euttge] as opposed to [eqit_trans_clo]
+     capturing closure under [eq_itree] and [eutt] at the same time, since it's
+     the only one we need.
+   *)
 
   (* A transitivity functor *)
-  Variant eqit_trans_clo  (b1 b2 b1' b2' : bool)  (r : itree E1 R1 -> itree E2 R2 -> Prop) :
+  Variant euttge_trans_clo (r : itree E1 R1 -> itree E2 R2 -> Prop) :
     itree E1 R1 -> itree E2 R2 -> Prop :=
     eqit_trans_clo_intro t1 t2 t1' t2' RR1 RR2
-      (EQVl: eqit RR1 b1 b1' t1 t1')
-      (EQVr: eqit RR2 b2 b2' t2 t2')
-      (REL: r t1' t2')
-      (LERR1: forall x x' y, RR1 x x' -> RR x' y -> RR x y)
-      (LERR2: forall x y y', RR2 y y' -> RR x y' -> RR x y) :
-      eqit_trans_clo b1 b2 b1' b2' r t1 t2.
-  Hint Constructors eqit_trans_clo : core.
-  (* sets directionality *)
-  Definition eqitC_rutt b1 b2 := eqit_trans_clo b1 b2 false false.
-  Hint Unfold eqitC_rutt : core.
+                         (EQVl: euttge RR1 t1 t1')
+                         (EQVr: euttge RR2 t2 t2')
+                         (REL: r t1' t2')
+                         (LERR1: forall x x' y, RR1 x x' -> RR x' y -> RR x y)
+                         (LERR2: forall x y y', RR2 y y' -> RR x y' -> RR x y) :
+      euttge_trans_clo r t1 t2.
+  Hint Constructors euttge_trans_clo : core.
 
-  Lemma eqitC_rutt_mon b1 b2 r1 r2 t1 t2
-    (IN : eqitC_rutt b1 b2 r1 t1 t2)
-    (LE : r1 <2= r2) :
-    eqitC_rutt b1 b2 r2 t1 t2.
+  Lemma euttge_trans_clo_mon r1 r2 t1 t2
+        (IN : euttge_trans_clo r1 t1 t2)
+        (LE : r1 <2= r2) :
+    euttge_trans_clo r2 t1 t2.
   Proof.
     destruct IN; econstructor; eauto.
   Qed.
 
-  Hint Resolve eqitC_rutt_mon : paco.
+  Hint Resolve euttge_trans_clo_mon : paco.
 
-End eqitC_rutt.
+End euttge_trans_clo.
 
 (*replicate this proof for the models functor*)
-Lemma eqitC_rutt_wcompat (b1 b2 : bool) E1 E2 R1 R2 (REv : forall A B, E1 A -> E2 B -> Prop)
-      (RAns : forall A B, E1 A -> A -> E2 B -> B -> Prop ) (RR : R1 -> R2 -> Prop)
-     (vclo: (itree E1 R1 -> itree E2 R2 -> Prop) -> (itree E1 R1 -> itree E2 R2 -> Prop) )
-     (MON: monotone2 vclo)
-      (CMP: compose (eqitC_rutt RR b1 b2) vclo <3= compose vclo (eqitC_rutt RR b1 b2)) :
-  wcompatible2 (Rutt.rutt_ REv RAns RR vclo) (eqitC_rutt RR b1 b2).
+(* Validity of the up-to [euttge] principle *)
+Lemma euttge_trans_clo_wcompat E1 E2 R1 R2 (REv : forall A B, E1 A -> E2 B -> Prop)
+      (RAns : forall A B, E1 A -> A -> E2 B -> B -> Prop ) (RR : R1 -> R2 -> Prop) :
+  wcompatible2 (rutt_ REv RAns RR) (euttge_trans_clo RR).
 Proof.
   constructor; eauto with paco.
-  { red. intros. eapply eqitC_rutt_mon; eauto. }
+  { red. intros. eapply euttge_trans_clo_mon; eauto. }
   intros.
   destruct PR. punfold EQVl. punfold EQVr. unfold_eqit.
   hinduction REL before r; intros; clear t1' t2'.
@@ -177,44 +173,46 @@ Proof.
     remember (TauF m3) as y.
     hinduction EQVr before r; intros; subst; try inv Heqy; try inv CHECK; (try (constructor; eauto; fail)).
     pclearbot. constructor. gclo. econstructor; eauto with paco.
-  - remember (TauF t1) as x. red.
-    hinduction EQVl before r; intros; subst; try inv Heqx; try inv CHECK; (try (constructor; eauto; fail)).
-    pclearbot. punfold REL. constructor. eapply IHREL; eauto.
-  - remember (TauF t2) as y. red.
-    hinduction EQVr before r; intros; subst; try inv Heqy; try inv CHECK; (try (constructor; eauto; fail)).
-    pclearbot. punfold REL. constructor. eapply IHREL; eauto.
   - remember (VisF e1 k1) as x. red.
     hinduction EQVl before r; intros; subst; try discriminate; try (constructor; eauto; fail).
     remember (VisF e2 k3) as y.
     hinduction EQVr before r; intros; subst; try discriminate; try (constructor; eauto; fail).
     dependent destruction Heqx.
     dependent destruction Heqy.
-    constructor; auto. intros. apply H0 in H1. pclearbot. eapply MON.
-    + eapply CMP. red. econstructor; eauto.
-    + intros. apply gpaco2_clo; auto.
+    constructor; auto. intros. apply H0 in H1. pclearbot.
+    apply gpaco2_clo.
+    econstructor; eauto.
+  - remember (TauF t1) as x. red.
+    hinduction EQVl before r; intros; subst; try inv Heqx; try inv CHECK; (try (constructor; eauto; fail)).
+    pclearbot. punfold REL. constructor. eapply IHREL; eauto.
+  - remember (TauF t2) as y. red.
+    hinduction EQVr before r; intros; subst; try inv Heqy; try inv CHECK; (try (constructor; eauto; fail)).
+    pclearbot. punfold REL. constructor. eapply IHREL; eauto.
 Qed.
 
-Definition eqitC_rutt_wcompat' := eqitC_rutt_wcompat true true.
+#[export] Hint Resolve euttge_trans_clo_wcompat : paco.
 
-Hint Resolve (eqitC_rutt_wcompat') : paco.
-
-Global Instance grutt_cong_eqit {R1 R2 : Type} {E1 E2 : Type -> Type} {REv : forall A B, E1 A -> E2 B -> Prop}
-      {RAns : forall A B, E1 A -> A -> E2 B -> B -> Prop} {RR1 RR2} {RS : R1 -> R2 -> Prop} r rg
-      (LERR1: forall x x' y, (RR1 x x': Prop) -> (RS x' y: Prop) -> RS x y)
+(* The validity of the up-to [euttge] entails we can rewrite under [euttge]
+   and hence also [eq_itree] during coinductive proofs of [rutt]
+*)
+#[global] Instance grutt_cong_eqit {R1 R2 : Type} {E1 E2 : Type -> Type} {REv : forall A B, E1 A -> E2 B -> Prop}
+       {RAns : forall A B, E1 A -> A -> E2 B -> B -> Prop} {RR1 RR2} {RS : R1 -> R2 -> Prop} r rg
+       (LERR1: forall x x' y, (RR1 x x': Prop) -> (RS x' y: Prop) -> RS x y)
        (LERR2: forall x y y', (RR2 y y': Prop) -> RS x y' -> RS x y) :
-    Proper (eq_itree RR1 ==> eq_itree RR2 ==> flip impl)
-         (gpaco2 (Rutt.rutt_ REv RAns RS id) (eqitC_rutt RS true true) r rg).
+  Proper (eq_itree RR1 ==> eq_itree RR2 ==> flip impl)
+         (gpaco2 (rutt_ REv RAns RS) (euttge_trans_clo RS) r rg).
 Proof.
   repeat intro. gclo. econstructor; eauto;
-  try eapply eqit_mon; try apply H; try apply H0; auto.
+    try eapply eqit_mon; try apply H; try apply H0; auto.
 Qed.
 
 Global Instance grutt_cong_euttge {R1 R2 : Type} {E1 E2 : Type -> Type} {REv : forall A B, E1 A -> E2 B -> Prop}
-      {RAns : forall A B, E1 A -> A -> E2 B -> B -> Prop} {RR1 RR2} {RS : R1 -> R2 -> Prop} r rg
-      (LERR1: forall x x' y, (RR1 x x': Prop) -> (RS x' y: Prop) -> RS x y)
+       {RAns : forall A B, E1 A -> A -> E2 B -> B -> Prop} {RR1 RR2} {RS : R1 -> R2 -> Prop} r rg
+       (LERR1: forall x x' y, (RR1 x x': Prop) -> (RS x' y: Prop) -> RS x y)
        (LERR2: forall x y y', (RR2 y y': Prop) -> RS x y' -> RS x y) :
-    Proper (euttge RR1 ==> euttge RR2 ==> flip impl)
-         (gpaco2 (Rutt.rutt_ REv RAns RS id) (eqitC_rutt RS true true) r rg).
+  Proper (euttge RR1 ==> euttge RR2 ==> flip impl)
+         (gpaco2 (rutt_ REv RAns RS) (euttge_trans_clo RS) r rg).
 Proof.
   repeat intro. gclo. econstructor; eauto.
 Qed.
+ 
