theories/ITrace/ITracePreds.v
@@ -19,15 +19,15 @@ Local Open Scope monad_scope.
 
 (* Defines some useful predicates over ITraces *)
 
-Variant trace_forallF {E : Type -> Type} {R : Type} (F : itrace E R -> Prop) 
+Variant trace_forallF {E : Type -> Type} {R : Type} (F : itrace E R -> Prop)
         (PE : forall A, EvAns E A -> Prop) (PR : R -> Prop) : itrace' E R -> Prop :=
-| trace_forall_ret (r : R) : PR r -> trace_forallF F PE PR (RetF r)
-| trace_forall_tau (b : itrace E R) : F b -> trace_forallF F PE PR (TauF b)
-| trace_forall_vis {A : Type} (e : EvAns E A) (k : A -> itrace E R) :
+  | trace_forall_ret (r : R) : PR r -> trace_forallF F PE PR (RetF r)
+  | trace_forall_tau (b : itrace E R) : F b -> trace_forallF F PE PR (TauF b)
+  | trace_forall_vis {A : Type} (e : EvAns E A) (k : A -> itrace E R) :
     PE A e -> (forall (a :A), F (k a) ) -> trace_forallF F PE PR (VisF e k)
 .
 
-Hint Constructors trace_forallF.
+#[global] Hint Constructors trace_forallF : core.
 
 Definition trace_forall_ {E R} PE PR F (b : itrace E R) :=
   trace_forallF F PE PR (observe b).
@@ -37,12 +37,12 @@ Proof.
   repeat intro. red in IN. red. induction IN; auto.
 Qed.
 
-Hint Resolve trace_forall_monot : paco.
+#[global] Hint Resolve trace_forall_monot : paco.
 
 Definition trace_forall {E R} PE PR := paco1 (@trace_forall_ E R PE PR) bot1.
 
 Lemma trace_forall_proper_aux: forall (E : Type -> Type) (R : Type) (PE : forall A : Type, EvAns E A -> Prop)
-                                  (PR : R -> Prop) (b1 b2 : itree (EvAns E) R),
+                                 (PR : R -> Prop) (b1 b2 : itree (EvAns E) R),
     (b1 ≈ b2) -> trace_forall PE PR b1 -> trace_forall PE PR b2.
 Proof.
   intros E R PE PR. pcofix CIH. intros b1 b2 Heutt Hforall.
@@ -56,14 +56,12 @@ Proof.
   - constructor. left. pfold. red. apply IHHeutt. auto.
 Qed.
 
-Global Instance trace_forall_proper_eutt {E R PE PR} : Proper (eutt eq ==> iff) (@trace_forall E R PE PR).
+#[global] Instance trace_forall_proper_eutt {E R PE PR} : Proper (eutt eq ==> iff) (@trace_forall E R PE PR).
 Proof.
   intros b1 b2 Heutt. split; intros.
   - eapply trace_forall_proper_aux; eauto.
   - symmetry in Heutt. eapply trace_forall_proper_aux; eauto.
 Qed.
-    
-      
 
 Lemma forall_spin : forall E R PE PR, trace_forall PE PR (@ITree.spin (EvAns E) R).
 Proof.
@@ -72,16 +70,16 @@ Proof.
 Qed.
 
 Inductive trace_inf_oftenF {E : Type -> Type} {R : Type} (PE : forall A, EvAns E A -> Prop)
-        (F : itrace E R -> Prop) : itrace' E R -> Prop :=
-| trace_inf_often_tau (b : itrace E R) : trace_inf_oftenF PE F (observe b) -> 
-                                             trace_inf_oftenF PE F (TauF b)
-| trace_inf_often_vis_neg (e : EvAns E unit) (k : unit -> itrace E R) : 
-    trace_inf_oftenF PE F (observe (k tt)) -> trace_inf_oftenF PE F (VisF e k)
-| trace_inf_often_vis_pos (e : EvAns E unit) (k : unit -> itrace E R) : 
-    F (k tt) -> PE unit e -> trace_inf_oftenF PE F (VisF e k)
+          (F : itrace E R -> Prop) : itrace' E R -> Prop :=
+| trace_inf_often_tau (b : itrace E R) : trace_inf_oftenF PE F (observe b) ->
+                                         trace_inf_oftenF PE F (TauF b)
+| trace_inf_often_vis_neg (e : EvAns E unit) (k : unit -> itrace E R) :
+  trace_inf_oftenF PE F (observe (k tt)) -> trace_inf_oftenF PE F (VisF e k)
+| trace_inf_often_vis_pos (e : EvAns E unit) (k : unit -> itrace E R) :
+  F (k tt) -> PE unit e -> trace_inf_oftenF PE F (VisF e k)
 .
 
-Hint Constructors trace_inf_oftenF.
+#[global] Hint Constructors trace_inf_oftenF : core.
 
 Definition trace_inf_often_ {E R} PE F (b : itrace E R) :=
   trace_inf_oftenF PE F (observe b).
@@ -91,17 +89,17 @@ Proof.
   repeat intro. red in IN. red. induction IN; auto.
 Qed.
 
-Hint Resolve trace_inf_often_monot : paco.
+#[global] Hint Resolve trace_inf_often_monot : paco.
 
 Definition trace_inf_often {E R} PE := paco1 (@trace_inf_often_ E R PE) bot1.
 
 Inductive front_and_last {E : Type -> Type} {R : Type} (PEF : forall A, EvAns E A -> Prop)
           (PEL : forall A, EvAns E A -> Prop) (PR : R -> Prop) : itrace E R -> Prop :=
 | front_and_last_base (e : EvAns E unit) (r : R) (b : itree (EvAns E) R) :
-    b ≈ Vis e (fun u => Ret r) -> PEL unit e -> PR r -> front_and_last PEF PEL PR b
-  | front_and_last_cons (e : EvAns E unit) (k : unit -> itrace E R) (b : itree (EvAns E) R ) :
-      b ≈ Vis e k -> PEF unit e -> front_and_last PEF PEL PR (k tt) -> front_and_last PEF PEL PR b
-      
+  b ≈ Vis e (fun u => Ret r) -> PEL unit e -> PR r -> front_and_last PEF PEL PR b
+| front_and_last_cons (e : EvAns E unit) (k : unit -> itrace E R) (b : itree (EvAns E) R ) :
+  b ≈ Vis e k -> PEF unit e -> front_and_last PEF PEL PR (k tt) -> front_and_last PEF PEL PR b
+
 .
 
 Lemma fal_proper_aux: forall (E : Type -> Type) (R : Type) (PEF PEL : forall A : Type, EvAns E A -> Prop)
@@ -115,62 +113,63 @@ Proof.
   - eapply front_and_last_cons; eauto. rewrite <- Heutt. auto.
 Qed.
 
-Global Instance front_and_last_proper_eutt {E R PEF PEL PR} : Proper (eutt eq ==> iff) (@front_and_last E R PEF PEL PR).
+#[global] Instance front_and_last_proper_eutt {E R PEF PEL PR} :
+  Proper (eutt eq ==> iff) (@front_and_last E R PEF PEL PR).
 Proof.
   intros b1 b2 Heutt. split; intros.
   - eapply fal_proper_aux; eauto.
   - symmetry in Heutt. eapply fal_proper_aux; eauto.
 Qed.
-     
-Section StateMachine.
-(*Note that this state machine definition is not able to deal with empty event parameter types*)
-(*Nor can it encode predicates that can accept silent divergence under certain conditions *)
-(*Pretty sure it could be extended to handle that,but that is a job for another day*)
-Context {E : Type -> Type}.
-Context {R : Type}.
-Context (EvTrans : forall A, E A -> A -> forall B, E B -> B -> Prop).
-Context (RetTrans : forall A, E A -> A -> R -> Prop).
 
-Inductive state_machineF (PEv : forall A, E A -> A -> Prop) (PRet : R -> Prop) 
-          (F : (forall A, E A -> A -> Prop) -> (R -> Prop) -> itrace E R -> Prop) : itrace' E R -> Prop :=
+Section StateMachine.
+  (*Note that this state machine definition is not able to deal with empty event parameter types*)
+  (*Nor can it encode predicates that can accept silent divergence under certain conditions *)
+  (*Pretty sure it could be extended to handle that,but that is a job for another day*)
+  Context {E : Type -> Type}.
+  Context {R : Type}.
+  Context (EvTrans : forall A, E A -> A -> forall B, E B -> B -> Prop).
+  Context (RetTrans : forall A, E A -> A -> R -> Prop).
+
+  Inductive state_machineF (PEv : forall A, E A -> A -> Prop) (PRet : R -> Prop)
+            (F : (forall A, E A -> A -> Prop) -> (R -> Prop) -> itrace E R -> Prop) : itrace' E R -> Prop :=
   | smRet r : PRet r -> state_machineF PEv PRet F (RetF r)
   | smTau t : state_machineF PEv PRet F (observe t) -> state_machineF PEv PRet F (TauF t)
-  | smVis A (e : E A) (a : A) (k : unit -> itrace E R) : 
-      PEv A e a -> F (EvTrans A e a) (RetTrans A e a) (k tt) -> state_machineF PEv PRet F (VisF (evans A e a) k)
-.
+  | smVis A (e : E A) (a : A) (k : unit -> itrace E R) :
+    PEv A e a -> F (EvTrans A e a) (RetTrans A e a) (k tt) -> state_machineF PEv PRet F (VisF (evans A e a) k)
+  .
 
-Hint Constructors state_machineF.
+  Hint Constructors state_machineF : core.
 
-Definition state_machine_ F PEv PRet (tr : itrace E R) :=
-  state_machineF PEv PRet F (observe tr).
+  Definition state_machine_ F PEv PRet (tr : itrace E R) :=
+    state_machineF PEv PRet F (observe tr).
 
-Lemma monotone_state_machine : monotone3 state_machine_.
-Proof.
-  red. intros. red. red in IN. induction IN; auto.
-Qed.
-Hint Resolve trace_inf_often_monot : paco.
-Definition state_machine PEv PRet (tr : itrace E R) :  Prop := paco3 (state_machine_) bot3 PEv PRet tr.
+  Lemma monotone_state_machine : monotone3 state_machine_.
+  Proof.
+    red. intros. red. red in IN. induction IN; auto.
+  Qed.
+  Hint Resolve trace_inf_often_monot : paco.
+  Definition state_machine PEv PRet (tr : itrace E R) :  Prop := paco3 (state_machine_) bot3 PEv PRet tr.
 
-Lemma state_machine_proper_aux : forall PEv PRet (t1 t2 : itrace E R), 
-    (t1 ≈ t2) -> state_machine PEv PRet t1 -> state_machine PEv PRet t2.
-Proof.
-  pcofix CIH. intros PEV PREt t1 t2 Heutt Hsm. pfold. red.
-  punfold Hsm; try apply monotone_state_machine.
-  punfold Heutt. red in Heutt. red in Hsm. 
-  induction Hsm.
-  - remember (RetF r0) as ot1. induction Heutt; subst; auto; try discriminate.
-    injection Heqot1; intros; subst; auto.
-  - apply IHHsm. pstep_reverse. assert (Tau t ≈ t2); auto.
-    rewrite tau_eutt in H. auto.
-  - remember (VisF (evans A e a) k ) as ot1. induction Heutt; subst; auto; try discriminate.
-    injection Heqot1; intros; subst. dependent destruction H1.
-    subst. constructor; auto. right. pclearbot. eapply CIH; eauto.
-    destruct H0; tauto.
-Qed.
+  Lemma state_machine_proper_aux : forall PEv PRet (t1 t2 : itrace E R),
+      (t1 ≈ t2) -> state_machine PEv PRet t1 -> state_machine PEv PRet t2.
+  Proof.
+    pcofix CIH. intros PEV PREt t1 t2 Heutt Hsm. pfold. red.
+    punfold Hsm; try apply monotone_state_machine.
+    punfold Heutt. red in Heutt. red in Hsm.
+    induction Hsm.
+    - remember (RetF r0) as ot1. induction Heutt; subst; auto; try discriminate.
+      injection Heqot1; intros; subst; auto.
+    - apply IHHsm. pstep_reverse. assert (Tau t ≈ t2); auto.
+      rewrite tau_eutt in H. auto.
+    - remember (VisF (evans A e a) k ) as ot1. induction Heutt; subst; auto; try discriminate.
+      injection Heqot1; intros; subst. dependent destruction H1.
+      subst. constructor; auto. right. pclearbot. eapply CIH; eauto.
+      destruct H0; tauto.
+  Qed.
 
-Global Instance state_machine_proper_eutt {PEv PRet} : Proper (eutt eq ==> iff) (@state_machine PEv PRet).
-Proof.
-  intros t1 t2 Heutt. split; intros; try eapply state_machine_proper_aux; eauto; symmetry; auto.
-Qed.
+  #[global] Instance state_machine_proper_eutt {PEv PRet} : Proper (eutt eq ==> iff) (@state_machine PEv PRet).
+  Proof.
+    intros t1 t2 Heutt. split; intros; try eapply state_machine_proper_aux; eauto; symmetry; auto.
+  Qed.
 
 End StateMachine.
