theories/ITrace/ITracePrefix.v
@@ -23,33 +23,33 @@ Local Open Scope monad_scope.
 (* Defines and explores a notion of traces being prefixes of other traces *)
 
 Inductive trace_prefixF {E : Type -> Type} {R S : Type} (F : itrace E R -> itrace E S -> Prop) : itrace' E R -> itrace' E S ->  Prop :=
-  | ret_prefix (r : R) (b : itrace E S) : trace_prefixF F (RetF r) (observe b)
-  | tau_prefix (br : itrace E R) (bs : itrace E S) : F br bs -> trace_prefixF F (TauF br) (TauF bs)
-  | tau_r_prefix (br : itrace E R) (obs : itrace' E S) : trace_prefixF F (observe br) obs -> trace_prefixF F (TauF br) obs
-  | tau_l_prefix (obr : itrace' E R) (bs : itrace E S) : trace_prefixF F (obr) (observe bs) -> trace_prefixF F (obr) (TauF bs)
-  | tau_vis_empty {A : Type} (e : E A) (H: A -> void) (kr : void -> itrace E R) (ks : void -> itrace E S) : 
-      trace_prefixF F (VisF (evempty A H e) kr) (VisF (evempty A H e) ks )
-  | tau_vis_ans {A : Type} (e : E A) (ans : A) (kr : unit -> itrace E R) (ks : unit -> itrace E S) :
-      F (kr tt) (ks tt) -> trace_prefixF F (VisF (evans A e ans) kr ) (VisF (evans A e ans) ks)
+| ret_prefix (r : R) (b : itrace E S) : trace_prefixF F (RetF r) (observe b)
+| tau_prefix (br : itrace E R) (bs : itrace E S) : F br bs -> trace_prefixF F (TauF br) (TauF bs)
+| tau_r_prefix (br : itrace E R) (obs : itrace' E S) : trace_prefixF F (observe br) obs -> trace_prefixF F (TauF br) obs
+| tau_l_prefix (obr : itrace' E R) (bs : itrace E S) : trace_prefixF F (obr) (observe bs) -> trace_prefixF F (obr) (TauF bs)
+| tau_vis_empty {A : Type} (e : E A) (H: A -> void) (kr : void -> itrace E R) (ks : void -> itrace E S) :
+  trace_prefixF F (VisF (evempty A H e) kr) (VisF (evempty A H e) ks )
+| tau_vis_ans {A : Type} (e : E A) (ans : A) (kr : unit -> itrace E R) (ks : unit -> itrace E S) :
+  F (kr tt) (ks tt) -> trace_prefixF F (VisF (evans A e ans) kr ) (VisF (evans A e ans) ks)
 .
 
-Hint Constructors trace_prefixF.
+#[global] Hint Constructors trace_prefixF : core.
 
 Definition trace_prefix_ {E R S} F (br : itrace E R) (bs : itrace E S) := trace_prefixF F (observe br) (observe bs).
 
-Hint Unfold trace_prefix_.
+#[global] Hint Unfold trace_prefix_ : core.
 
 Lemma trace_prefix_monot {E R S} : monotone2 (@trace_prefix_ E R S).
 Proof.
   repeat intro. red. red in IN. induction IN; eauto.
 Qed.
 
-Hint Resolve trace_prefix_monot : paco.
+#[global] Hint Resolve trace_prefix_monot : paco.
 
 Definition trace_prefix {E R S} : itrace E R -> itrace E S -> Prop := paco2 trace_prefix_ bot2.
 
-Lemma prefix_vis : forall E R S A (e : E A) (ans : A) (k : unit -> itrace E R) (t : itrace E S), 
-                     trace_prefix (Vis (evans _ e ans) k ) t -> exists k', (t ≈ Vis (evans _ e ans) k' )%itree.
+Lemma prefix_vis : forall E R S A (e : E A) (ans : A) (k : unit -> itrace E R) (t : itrace E S),
+    trace_prefix (Vis (evans _ e ans) k ) t -> exists k', (t ≈ Vis (evans _ e ans) k' )%itree.
 Proof.
   intros E R S A e ans k t Hbp. punfold Hbp. red in Hbp. cbn in *.
   dependent induction Hbp.
@@ -67,7 +67,7 @@ Proof.
 Qed.
 
 Lemma trace_prefix_proper_aux_vis: forall (E : Type -> Type) (S R : Type)
-                                  (t1 : itree (EvAns E) R) (b2 : itrace E R),
+                                     (t1 : itree (EvAns E) R) (b2 : itrace E R),
     eqitF eq true true id
           (upaco2 (eqit_ eq true true id) bot2)
           (observe t1) (observe b2) ->
@@ -75,13 +75,13 @@ Lemma trace_prefix_proper_aux_vis: forall (E : Type -> Type) (S R : Type)
       (X : Type) (e : EvAns E X)
       (k : X -> itree (EvAns E) S),
       trace_prefixF (upaco2 trace_prefix_ bot2)
-                     (observe t1) (VisF e k) ->
+                    (observe t1) (VisF e k) ->
       (forall (b1 b2 : itrace E R)
          (b : itrace E S),
           (b1 ≈ b2) ->
           trace_prefix b1 b -> r b2 b) ->
-        trace_prefixF (upaco2 trace_prefix_ r)
-        (observe b2) (VisF e k).
+      trace_prefixF (upaco2 trace_prefix_ r)
+                    (observe b2) (VisF e k).
 Proof.
   intros E S R t1 b2 Heutt r X e k H0 CIH.
   dependent induction H0.
@@ -103,7 +103,7 @@ Lemma trace_prefix_tau_inv:
   forall (E : Type -> Type) (S R : Type)
     (m1 : itree (EvAns E) R) (t : itree (EvAns E) S),
     trace_prefixF (upaco2 trace_prefix_ bot2)
-                   (TauF m1) (TauF t) -> trace_prefix m1 t.
+                  (TauF m1) (TauF t) -> trace_prefix m1 t.
 Proof.
   intros E S R m1 t Hbp.
   dependent induction  Hbp.
@@ -126,9 +126,9 @@ Proof.
   pfold. red. punfold Heutt. red in Heutt. punfold Hbp. red in Hbp.
   dependent induction Heutt.
   - rewrite <- x. constructor.
-  - rewrite <- x. rewrite <- x0 in Hbp. clear x0 x. pclearbot. 
+  - rewrite <- x. rewrite <- x0 in Hbp. clear x0 x. pclearbot.
     destruct (observe b) eqn : Heqb.
-    + inv Hbp. constructor. dependent induction  H0. 
+    + inv Hbp. constructor. dependent induction  H0.
       * apply simpobs in x0. assert (m1 ≈ m2); auto.
         rewrite x0 in H. clear x x0 Heqb CIH REL.
         punfold H. red in H. cbn in *. dependent induction H.
@@ -138,14 +138,14 @@ Proof.
         apply simpobs in x. assert (m1 ≈ m2); auto.
         rewrite x in H. rewrite tau_eutt in H. auto.
     + constructor. right. eapply CIH; eauto. eapply trace_prefix_tau_inv; eauto.
-    + constructor. clear Heqb. inv Hbp. dependent induction H0. 
+    + constructor. clear Heqb. inv Hbp. dependent induction H0.
       * apply simpobs in x0. assert (m1 ≈ m2); auto.
         rewrite x0 in H. punfold H. red in H. cbn in *.
         dependent induction H.
-       ++ rewrite <- x. apply trace_prefix_ret.
-       ++ rewrite <- x. constructor. eapply IHeqitF; eauto.
-          assert (m1 ≈ m2); auto.
-          apply simpobs in x. rewrite x in H0. rewrite tau_eutt in H0. auto.
+        ++ rewrite <- x. apply trace_prefix_ret.
+        ++ rewrite <- x. constructor. eapply IHeqitF; eauto.
+           assert (m1 ≈ m2); auto.
+           apply simpobs in x. rewrite x in H0. rewrite tau_eutt in H0. auto.
       * eapply IHtrace_prefixF; auto.
         assert (m1 ≈ m2); auto. apply simpobs in x.
         rewrite x in H. rewrite tau_eutt in H. auto.
@@ -161,7 +161,7 @@ Proof.
         rewrite x in H0. punfold H0. red in H0. cbn in *.
         dependent induction H0.
         ++ rewrite <- x. constructor. right. pclearbot. eapply CIH; eauto.
-        ++ rewrite <- x. constructor. eapply IHeqitF; eauto. 
+        ++ rewrite <- x. constructor. eapply IHeqitF; eauto.
            assert (m1 ≈ m2); auto.
            apply simpobs in x. rewrite x in H1. rewrite tau_eutt in H1. auto.
   - rewrite <- x. rewrite <- x0 in Hbp. clear x x0. pclearbot.
@@ -177,9 +177,9 @@ Proof.
         dependent induction  Heutt.
         ++ rewrite <- x. apply trace_prefix_ret.
         ++ rewrite <- x. constructor. eapply IHHeutt; eauto.
-       * eapply IHtrace_prefixF; auto.
-         assert (t1 ≈ b2); auto.
-         apply simpobs in x. rewrite x in H. rewrite tau_eutt in H. punfold H.
+      * eapply IHtrace_prefixF; auto.
+        assert (t1 ≈ b2); auto.
+        apply simpobs in x. rewrite x in H. rewrite tau_eutt in H. punfold H.
     + constructor. eapply IHHeutt; eauto. pstep_reverse. eapply trace_prefix_tau_inv; eauto.
     + clear IHHeutt. inv Hbp. eapply trace_prefix_proper_aux_vis; eauto.
   - rewrite <- x. constructor. eapply IHHeutt; eauto.
@@ -187,11 +187,11 @@ Qed.
 
 Lemma trace_prefixF_tau_inv_r:
   forall (E : Type -> Type) (S R : Type)
-    (t1 : itree (EvAns E) S) (b : itrace E R),
+         (t1 : itree (EvAns E) S) (b : itrace E R),
     trace_prefixF (upaco2 trace_prefix_ bot2)
-                   (observe b) (TauF t1) ->
+                  (observe b) (TauF t1) ->
     trace_prefixF (upaco2 trace_prefix_ bot2)
-                   (observe b) (observe t1).
+                  (observe b) (observe t1).
 Proof.
   intros E S R t1 b Hbp.
   dependent induction  Hbp.
@@ -200,22 +200,22 @@ Proof.
   - rewrite <- x. constructor. eapply IHHbp; eauto.
   - auto.
 Qed.
-  
+
 Lemma trace_prefixF_vis_l:
   forall (E : Type -> Type) (S R : Type)
-    (m1 m2 : itree (EvAns E) S),
+         (m1 m2 : itree (EvAns E) S),
     paco2 (eqit_ eq true true id) bot2 m1 m2 ->
     forall (r : itrace E R -> itrace E S -> Prop)
-      (X : Type) (e : EvAns E X)
-      (k : X -> itree (EvAns E) R),
+           (X : Type) (e : EvAns E X)
+           (k : X -> itree (EvAns E) R),
       trace_prefixF (upaco2 trace_prefix_ bot2)
-                     (VisF e k) (observe m1) ->
+                    (VisF e k) (observe m1) ->
       (forall (b : itrace E R)
-         (b1 b2 : itrace E S),
+              (b1 b2 : itrace E S),
           (b1 ≈ b2) ->
           trace_prefix b b1 -> r b b2 ) ->
-      trace_prefixF (upaco2 trace_prefix_ r) 
-                     (VisF e k) (observe m2).
+      trace_prefixF (upaco2 trace_prefix_ r)
+                    (VisF e k) (observe m2).
 Proof.
   intros E S R m1 m2 REL r X e k H1 CIH.
   punfold REL. red in REL.
@@ -228,7 +228,7 @@ Proof.
     + rewrite <- x. constructor.
     + rewrite <- x. constructor. eapply IHREL; eauto.
   - pclearbot. rewrite <- x in REL. dependent induction REL.
-    + rewrite <- x. constructor. right. pclearbot. eapply CIH; eauto. 
+    + rewrite <- x. constructor. right. pclearbot. eapply CIH; eauto.
     + rewrite <- x. constructor. eapply IHREL; eauto.
 Qed.
 
@@ -254,8 +254,8 @@ Proof.
   - eapply IHHeutt; auto. rewrite <- x in Hbp. eapply trace_prefixF_tau_inv_r; eauto.
   - rewrite <- x. constructor. eapply IHHeutt; eauto.
 Qed.
-  
-Instance trace_prefix_proper {E R S} : Proper (eutt eq ==> eutt eq ==> iff) (@trace_prefix E R S).
+
+#[global] Instance trace_prefix_proper {E R S} : Proper (eutt eq ==> eutt eq ==> iff) (@trace_prefix E R S).
 Proof.
   repeat intro. split; intros.
   - eapply trace_prefix_proper_l; eauto.
@@ -266,9 +266,9 @@ Proof.
 Qed.
 
 Inductive ind_comb {E R S} : itrace E R -> itrace E S -> itrace E S -> Prop :=
-  | left_ret_comb (r : R) b1 b2 b : (b1 ≈ Ret r)%itree -> (b2 ≈ b)%itree -> ind_comb b1 b2 b
-  | left_vis_comb {A : Type} (e : E A) (ans : A) (k1 : unit -> itrace E R) (k2 : unit -> itrace E S) b1 b2 b 
-    : (b1 ≈ Vis (evans _ e ans) k1) -> (b ≈ (Vis (evans _ e ans) k2 ))%itree -> ind_comb (k1 tt) b2 (k2 tt) -> 
+| left_ret_comb (r : R) b1 b2 b : (b1 ≈ Ret r)%itree -> (b2 ≈ b)%itree -> ind_comb b1 b2 b
+| left_vis_comb {A : Type} (e : E A) (ans : A) (k1 : unit -> itrace E R) (k2 : unit -> itrace E S) b1 b2 b
+  : (b1 ≈ Vis (evans _ e ans) k1) -> (b ≈ (Vis (evans _ e ans) k2 ))%itree -> ind_comb (k1 tt) b2 (k2 tt) ->
     ind_comb b1 b2 b.
 
 
@@ -282,14 +282,15 @@ Proof.
 Qed.
 
 Inductive trace_prefix_ind {E R S} : itrace E R -> itrace E S -> Prop :=
-  | left_ret_bp (r : R) b1 b2 : (b1 ≈ Ret r)%itree -> trace_prefix_ind b1 b2
-  | left_vis_bp {A : Type} (e : E A) (ans : A) (k1 : unit -> itrace E R) (k2 : unit -> itrace E S) b1 b2 :
-      (b1 ≈ Vis (evans _ e ans) k1)%itree -> (b2 ≈ Vis (evans _ e ans) k2 )%itree -> trace_prefix_ind (k1 tt) (k2 tt) ->
-      trace_prefix_ind b1 b2
+| left_ret_bp (r : R) b1 b2 : (b1 ≈ Ret r)%itree -> trace_prefix_ind b1 b2
+| left_vis_bp {A : Type} (e : E A) (ans : A) (k1 : unit -> itrace E R) (k2 : unit -> itrace E S) b1 b2 :
+  (b1 ≈ Vis (evans _ e ans) k1)%itree -> (b2 ≈ Vis (evans _ e ans) k2 )%itree -> trace_prefix_ind (k1 tt) (k2 tt) ->
+  trace_prefix_ind b1 b2
 .
 
-Lemma trace_prefix_ind_comb : forall E R S (b1 : itrace E R) (b2 : itrace E S), trace_prefix_ind b1 b2 ->
-                                                                          exists b3, ind_comb b1 b3 b2.
+Lemma trace_prefix_ind_comb : forall E R S (b1 : itrace E R) (b2 : itrace E S),
+    trace_prefix_ind b1 b2 ->
+    exists b3, ind_comb b1 b3 b2.
 Proof.
   intros E R S b1 b2 Hpre. induction Hpre.
   - exists b2. econstructor; eauto. reflexivity.
@@ -297,14 +298,15 @@ Proof.
     exists b3. eapply left_vis_comb; eauto.
 Qed.
 
-Lemma trace_prefix_ind_bind : forall E R S (b1 : itrace E R) (b2 : itrace E S), trace_prefix_ind b1 b2 -> 
-  exists g, (ITree.bind b1 g ≈ b2)%itree.
+Lemma trace_prefix_ind_bind : forall E R S (b1 : itrace E R) (b2 : itrace E S),
+    trace_prefix_ind b1 b2 ->
+    exists g, (ITree.bind b1 g ≈ b2)%itree.
 Proof.
   intros. apply trace_prefix_ind_comb in H. destruct H as [b3 Hb3].
   apply ind_comb_bind in Hb3. exists (fun _ => b3). auto.
 Qed.
 
-Lemma converge_trace_prefix : forall E R S (b1 : itrace E R) (b2 : itrace E S) (r : R), 
+Lemma converge_trace_prefix : forall E R S (b1 : itrace E R) (b2 : itrace E S) (r : R),
     trace_prefix b1 b2 -> may_converge r b1 -> trace_prefix_ind b1 b2.
 Proof.
   intros E R S b1 b2 r Hbp Hconv. generalize dependent b2. induction Hconv; intros.
@@ -325,7 +327,7 @@ Proof.
   - inv Hdiv.
   - constructor. inv Hdiv. pclearbot. right. apply CIH; auto.
   - constructor; auto. apply IHHbf. pstep_reverse. inv Hdiv. pclearbot. auto.
-  - constructor; auto. 
+  - constructor; auto.
   - constructor. intuition.
   - pclearbot. constructor. intros. right. pclearbot. inv Hdiv. ddestruction; subst.
     pclearbot. destruct v. apply CIH; auto. apply H1.
@@ -338,7 +340,7 @@ Proof.
   - destruct H0 as [r Hconv]. eapply converge_trace_prefix in Hconv; eauto.
     apply trace_prefix_ind_bind. auto.
   - eapply trace_prefix_div in H0 as Heuttdiv; eauto.
-    exists (fun _ => ITree.spin). apply eutt_div_subrel. apply eutt_div_sym. 
+    exists (fun _ => ITree.spin). apply eutt_div_subrel. apply eutt_div_sym.
     eapply div_bind_nop with (f := (fun _ => ITree.spin) ) in H0 as H1.
     eapply eutt_div_trans; try apply H1. apply eutt_div_sym. auto.
 Qed.
